new/index.v
@@ -1,0 +1,110 @@
+Require Import braun log insert util.
+Require Import Arith Arith.Even Arith.Div2 List.
+Require Import Program.
+Require Import Omega.
+
+Section index.
+  Variable A : Set.
+
+  Inductive IndexR : bin_tree A -> nat -> A -> Prop :=
+    | IR_zero :
+        forall x s t,
+          IndexR (bt_node x s t) 0 x
+    | IR_left :
+        forall x s t i y,
+          IndexR s i y ->
+          IndexR (bt_node x s t) (2 * i + 1) y
+    | IR_right :
+        forall x s t i y,
+          IndexR t i y ->
+          IndexR (bt_node x s t) (2 * i + 2) y.
+  Hint Constructors IndexR.
+
+  Theorem index_dec :
+    forall bt i,
+      { x | IndexR bt i x } +
+      { forall x, ~ IndexR bt i x }.
+  Proof.
+    intros bt.
+    induction bt as [|x s IRs t IRt]; intros i.
+
+    right. intros x IR.
+    inversion IR.
+
+    destruct i as [|i].
+    left. eauto.
+
+    destruct (even_odd_dec i) as [E | O].
+
+    apply even_2n in E. 
+    destruct E as [k EQ]. subst.
+    unfold double.
+    replace (S (k + k)) with (2 * k + 1); try omega.
+    destruct (IRs k) as [[y IRs_k] | FAIL].
+    left. eauto.
+    right. intros y IR.
+    inversion IR; clear IR; subst; try omega.
+    replace i with k in *; try omega.
+    apply (FAIL y); auto.
+
+    apply odd_S2n in O.
+    destruct O as [k EQ]. subst.
+    unfold double.
+    replace (S (S (k + k))) with (2 * k + 2); try omega.
+    destruct (IRt k) as [[y IRt_k] | FAIL].
+    left. eauto.
+    right. intros y IR.
+    inversion IR; clear IR; subst; try omega.
+    replace i with k in *; try omega.
+    apply (FAIL y); auto.
+  Defined.
+
+  Theorem index_Braun :
+    forall bt n,
+      Braun bt n ->
+      forall i,
+        i < n ->
+        exists x,
+          IndexR bt i x.
+  Proof.
+    induction bt as [|x s Is t It];
+    intros n B i LT.
+
+    inversion B. omega.
+
+    inversion B; clear B; subst.
+    rename H2 into BP.
+    rename H4 into Bs.
+    rename H5 into Bt.
+    destruct i as [|i].
+    eauto.
+    destruct (even_odd_dec i) as [E | O].
+
+    apply even_2n in E. destruct E as [k EQ]; subst.
+    unfold double in *.
+    destruct (Is s_size Bs k) as [y IRs]; try omega.
+    replace (S (k + k)) with (2 * k + 1); try omega.
+    eauto.
+
+    apply odd_S2n in O. destruct O as [k EQ]; subst.
+    unfold double in *.
+    destruct (It t_size Bt k) as [y IRt]; try omega.
+    replace (S (S (k + k))) with (2 * k + 2); try omega.
+    eauto.
+  Qed.
+
+  Theorem index :
+    forall bt n,
+      Braun bt n ->
+      forall i,
+        i < n ->
+        { x | IndexR bt i x }.
+  Proof.
+    intros bt n B i LT.
+    destruct (index_dec bt i) as [OK | FAIL].
+    auto.
+    assert False; try tauto.
+    destruct (index_Braun bt n B i LT) as [y IR].
+    apply (FAIL y). auto.
+  Defined.
+End index.
